Redefined isort to make it stable for lt and le. Redefined is_sorted to accept isort. Not fully completed. To be removed if it does not eventually work.

main/SortingFun.v
@@ -45,13 +45,19 @@ Fixpoint is_sorted {A} (rel : A → A → bool) l :=
   match l with
   | [] => true
   | [a] => true
-  | a :: (b :: _) as la => (rel a b && is_sorted rel la)%bool
+  | a :: (b :: _) as la =>
+      if rel a b then is_sorted rel la
+      else if rel b a then false
+      else is_sorted rel la
   end.
 
 Fixpoint all_sorted A (rel : A → A → bool) a l :=
   match l with
   | [] => true
-  | b :: l' => (rel a b && all_sorted rel a l')%bool
+  | b :: l' =>
+      if rel a b then all_sorted rel a l'
+      else if rel b a then false
+      else all_sorted rel a l'
   end.
 
 Fixpoint is_strongly_sorted A (rel : A → A → bool) l :=
@@ -71,33 +77,50 @@ Proof.
 intros * Hs.
 cbn in Hs.
 destruct la as [| a']; [ easy | ].
-now apply Bool.andb_true_iff in Hs.
+unfold sorted in Hs |-*.
+remember (a' :: la) as lb; cbn in Hs; subst lb.
+destruct (rel a a'); [ easy | now destruct (rel a' a) ].
 Qed.
 
 Theorem sorted_strongly_sorted : ∀ A (rel : A → A → bool),
   transitive rel →
+  connected_relation rel →
   ∀ l, sorted rel l → strongly_sorted rel l.
 Proof.
-intros * Htra * Hs.
+intros * Htra Hcon * Hs.
 unfold sorted in Hs.
 unfold strongly_sorted.
 induction l as [| a]; [ easy | cbn ].
 rewrite IHl. 2: {
   destruct l as [| a']; [ easy | ].
-  now apply Bool.andb_true_iff in Hs.
+  now apply sorted_cons in Hs.
 }
 rewrite Bool.andb_true_r.
-clear IHl.
-induction l as [| b]; [ easy | cbn ].
+assert (H : is_sorted rel l = true) by now apply sorted_cons in Hs.
+specialize (IHl H); clear H.
+rename IHl into Hss.
+revert a Hs.
+induction l as [| b]; intros; [ easy | cbn ].
 remember (b :: l) as lb; cbn in Hs; subst lb.
-apply Bool.andb_true_iff in Hs.
-destruct Hs as (Hab, Hs).
-rewrite Hab; cbn.
-apply IHl; cbn in Hs |-*.
-destruct l as [| c]; [ easy | ].
-apply Bool.andb_true_iff in Hs.
-destruct Hs as (Hbc, Hs).
-now rewrite (Htra a b c Hab Hbc).
+cbn in Hss.
+apply Bool.andb_true_iff in Hss.
+destruct Hss as (Hbl, Hss).
+specialize (IHl Hss).
+remember (rel a b) as ab eqn:Hab; symmetry in Hab.
+destruct ab. {
+  apply IHl.
+  cbn in Hs |-*.
+  destruct l as [| c]; [ easy | ].
+  remember (rel b c) as bc eqn:Hbc; symmetry in Hbc.
+  destruct bc; [ now rewrite (Htra a b c Hab Hbc) | ].
+  remember (rel c b) as cb eqn:Hcb; symmetry in Hcb.
+  destruct cb; [ easy | ].
+  specialize (Hcon b c Hbc Hcb) as H; subst c.
+  now rewrite Hab.
+}
+remember (rel b a) as ba eqn:Hba; symmetry in Hba.
+destruct ba; [ easy | ].
+now specialize (Hcon a b Hab Hba) as H; subst b.
 Qed.
 
 Theorem strongly_sorted_sorted : ∀ A (rel : A → A → bool),
@@ -112,48 +135,57 @@ destruct Hs as (Ha, Hs).
 specialize (IHl Hs); cbn.
 destruct l as [| b]; [ easy | ].
 cbn in Ha.
-apply Bool.andb_true_iff in Ha.
-destruct Ha as (Hab, Ha).
-now rewrite Hab, IHl.
+remember (rel a b) as ab eqn:Hab; symmetry in Hab.
+destruct ab; [ easy | ].
+remember (rel b a) as ba eqn:Hba; symmetry in Hba.
+now destruct ba.
 Qed.
 
 Theorem all_sorted_forall : ∀ A (rel : A → _) a l,
   all_sorted rel a l = true
-  → ∀ b, b ∈ l → rel a b = true.
+  → ∀ b, b ∈ l → rel a b = true ∨ rel b a = false.
 Proof.
 intros * Hsal * Hb.
 induction l as [| c]; [ easy | ].
 destruct Hb as [Hb| Hb]. {
   subst c.
   cbn in Hsal.
-  now apply Bool.andb_true_iff in Hsal.
+  remember (rel a b) as ab eqn:Hab; symmetry in Hab.
+  destruct ab; [ now left | ].
+  remember (rel b a) as ba eqn:Hba; symmetry in Hba.
+  destruct ba; [ easy | now right ].
 }
 apply IHl; [ | easy ].
 cbn in Hsal.
-now apply Bool.andb_true_iff in Hsal.
+remember (rel a c) as ac eqn:Hac; symmetry in Hac.
+destruct ac; [ easy | ].
+remember (rel c a) as ca eqn:Hca; symmetry in Hca.
+now destruct ca.
 Qed.
 
 Theorem sorted_cons_iff : ∀ (A : Type) (rel : A → A → bool),
-  transitive rel
-  → ∀ a la,
-      sorted rel (a :: la) ↔
-      sorted rel la ∧ (∀ b, b ∈ la → rel a b = true).
+  transitive rel →
+  connected_relation rel →
+  ∀ a la,
+    sorted rel (a :: la) ↔
+    sorted rel la ∧ (∀ b, b ∈ la → rel a b = true ∨ rel b a = false).
 Proof.
-intros * Htra *.
+intros * Htra Hcon *.
 split; intros Hla. {
   split; [ now apply sorted_cons in Hla | ].
   intros b Hb.
   apply all_sorted_forall with (l := la); [ | easy ].
-  apply (sorted_strongly_sorted Htra) in Hla.
+  apply (sorted_strongly_sorted Htra Hcon) in Hla.
   unfold strongly_sorted in Hla; cbn in Hla.
   now apply Bool.andb_true_iff in Hla.
 } {
   destruct Hla as (Hs & Hla).
   unfold sorted; cbn.
   destruct la as [| b]; [ easy | ].
-  apply Bool.andb_true_iff.
-  split; [ | easy ].
-  now apply Hla; left.
+  specialize (Hla _ (or_introl eq_refl)) as H1.
+  destruct H1 as [H1| H1]; [ now rewrite H1 | ].
+  rewrite H1.
+  now destruct (rel a b).
 }
 Qed.
 
@@ -168,7 +200,12 @@ induction l as [| a]; intros; [ easy | ].
 cbn in Hi.
 apply Nat.succ_lt_mono in Hi.
 destruct l as [| b]; [ easy | ].
+unfold sorted in Hs.
 remember (b :: l) as l'; cbn in Hs |-*; subst l'.
+remember (rel a b) as ab eqn:Hab; symmetry in Hab.
+destruct ab. {
+  destruct i; [ easy | ].
+...
 apply Bool.andb_true_iff in Hs.
 destruct i; [ easy | ].
 now apply IHl.
@@ -359,6 +396,7 @@ Qed.
 
 (* isort: sort by insertion *)
 
+(*
 Fixpoint isort_insert {A} (rel : A → A → bool) a lsorted :=
   match lsorted with
   | [] => [a]
@@ -374,6 +412,20 @@ Fixpoint isort_loop {A} (rel : A → A → bool) lsorted l :=
   end.
 
 Definition isort {A} (rel : A → A → bool) := isort_loop rel [].
+*)
+
+Fixpoint isort {A} (rel : A → A → bool) l :=
+  match l with
+  | [] => []
+  | a :: l' =>
+      match isort rel l' with
+      | [] => [a]
+      | b :: l'' =>
+          if rel a b then a :: b :: l''
+          else if rel b a then b :: a :: l''
+          else a :: b :: l''
+      end
+  end.
 
 (* ssort: sort by selection *)
 
@@ -1360,6 +1412,7 @@ Qed.
 
 (* isort length *)
 
+(*
 Theorem isort_insert_length : ∀ A rel (a : A) lsorted,
   length (isort_insert rel a lsorted) = S (length lsorted).
 Proof.
@@ -1385,6 +1438,17 @@ Proof.
 intros.
 apply isort_loop_length.
 Qed.
+*)
+
+Theorem isort_length : ∀ A rel (l : list A), length (isort rel l) = length l.
+Proof.
+intros.
+induction l as [| a]; [ easy | cbn ].
+rewrite <- IHl.
+remember (isort rel l) as l' eqn:Hl'; symmetry in Hl'.
+destruct l' as [| b]; cbn; [ easy | ].
+destruct (rel a b); [ easy | now destruct (rel b a) ].
+Qed.
 
 (* ssort length *)
 
@@ -1408,6 +1472,7 @@ Qed.
 
 (* *)
 
+(*
 Theorem in_isort_insert_id : ∀ A (rel : A → _) a l,
   a ∈ isort_insert rel a l.
 Proof.
@@ -1547,9 +1612,11 @@ destruct x. {
   now apply permutation_app_comm.
 }
 Qed.
+*)
 
 (* in isort *)
 
+(*
 Theorem in_isort_insert : ∀ A (rel : A → A → bool) a b lsorted,
   a ∈ isort_insert rel b lsorted
   → a ∈ b :: lsorted.
@@ -1591,7 +1658,32 @@ intros * Ha.
 apply in_isort_loop in Ha.
 now destruct Ha.
 Qed.
+*)
 
+Theorem in_isort : ∀ A (rel : A → A → bool) a l, a ∈ isort rel l → a ∈ l.
+Proof.
+intros * Ha.
+induction l as [| b]; [ easy | ].
+cbn in Ha.
+remember (isort rel l) as l' eqn:Hl'; symmetry in Hl'.
+destruct l' as [| c]. {
+  destruct Ha as [Ha| ]; [ now left | easy ].
+}
+remember (rel b c) as bc eqn:Hbc; symmetry in Hbc.
+destruct bc. {
+  destruct Ha as [Ha| Ha]; [ now left | now right; apply IHl ].
+}
+remember (rel c b) as cb eqn:Hcb; symmetry in Hcb.
+destruct cb. {
+  destruct Ha as [Ha| Ha]. {
+    now subst c; right; apply IHl; left.
+  }
+  destruct Ha as [Ha| Ha]; [ now left | now right; apply IHl; right ].
+}
+destruct Ha as [Ha| Ha]; [ now left | now right; apply IHl ].
+Qed.
+
+(*
 Theorem isort_insert_trans_r : ∀ A (rel : A → _),
   transitive rel →
   ∀ a b la,
@@ -1627,6 +1719,7 @@ destruct (rel a a); [ now f_equal | ].
 f_equal.
 apply repeat_cons.
 Qed.
+*)
 
 (* *)
 
@@ -1866,6 +1959,7 @@ Qed.
 
 (* isort is sorted *)
 
+(*
 Theorem sorted_isort_insert : ∀ A (rel : A → _),
   total_relation rel →
   ∀ a lsorted,
@@ -1971,6 +2065,7 @@ symmetry.
 apply IHl.
 now rewrite <- app_assoc.
 Qed.
+*)
 
 Theorem select_first_sorted : ∀ A rel,
   transitive rel → ∀ (a b : A) la lb,
@@ -2850,6 +2945,7 @@ Qed.
 
 (* main *)
 
+(*
 Theorem isort_when_sorted : ∀ A (rel : A → _),
   transitive rel →
   ∀ l,
@@ -2858,6 +2954,27 @@ Theorem isort_when_sorted : ∀ A (rel : A → _),
 Proof.
 intros * Htra * Hs.
 now apply isort_loop_when_sorted.
+Qed.
+*)
+
+Theorem isort_when_sorted : ∀ A (rel : A → _) l,
+  sorted rel l → isort rel l = l.
+Proof.
+intros * Hs.
+induction l as [| a]; [ easy | cbn ].
+remember (isort rel l) as l' eqn:Hl'; symmetry in Hl'.
+destruct l' as [| b]. {
+  apply (f_equal length) in Hl'.
+  rewrite isort_length in Hl'.
+  now apply length_zero_iff_nil in Hl'; subst l.
+}
+rewrite <- IHl; [ | now apply sorted_cons in Hs ].
+remember (rel a b) as ab eqn:Hab; symmetry in Hab.
+destruct ab; [ easy | ].
+destruct (rel b a); [ | easy ].
+rewrite <- IHl in Hs; [ | now apply sorted_cons in Hs ].
+unfold sorted in Hs; cbn in Hs.
+now rewrite Hab in Hs.
 Qed.
 
 Theorem ssort_when_sorted : ∀ A (rel : A → _),
@@ -2895,6 +3012,7 @@ Qed.
 
 (* *)
 
+(*
 Theorem sorted_isort : ∀ A (rel : A → _),
   total_relation rel
   → ∀ l, sorted rel (isort rel l).
@@ -2903,6 +3021,39 @@ intros * Hto *.
 destruct l as [| a]; [ easy | cbn ].
 now apply sorted_isort_loop.
 Qed.
+*)
+
+Theorem sorted_isort : ∀ A (rel : A → _) l,
+  sorted rel (isort rel l).
+Proof.
+intros.
+induction l as [| a]; [ easy | cbn ].
+remember (isort rel l) as l' eqn:Hl'; symmetry in Hl'.
+destruct l' as [| b]; [ easy | ].
+remember (rel a b) as ab eqn:Hab; symmetry in Hab.
+destruct ab. {
+  unfold sorted.
+  remember (b :: l') as l''; cbn; subst l''.
+  now rewrite Hab, IHl.
+}
+remember (rel b a) as ba eqn:Hba; symmetry in Hba.
+destruct ba. {
+  unfold sorted.
+  remember (a :: l') as l''; cbn; subst l''.
+  rewrite Hba, Bool.andb_true_l.
+  unfold sorted in IHl; cbn in IHl |-*.
+  destruct l' as [| c]; [ easy | ].
+  apply Bool.andb_true_iff in IHl.
+  destruct IHl as (Hbc, IHl).
+  rewrite IHl, Bool.andb_true_r.
+  cbn in IHl.
+Print is_sorted.
+...
+destruct l as [| a]; [ easy | cbn ].
+now apply sorted_isort_loop.
+Qed.
+
+...
 
 Theorem sorted_ssort : ∀ A (rel : A → _),
   transitive rel →
@@ -3152,6 +3303,14 @@ intros a b c Hab Hbc.
 apply Nat.leb_le in Hab, Hbc.
 apply Nat.leb_le.
 now transitivity b.
+Qed.
+
+Theorem Nat_leb_connected : connected_relation Nat.leb.
+Proof.
+intros a b Hab Hba.
+apply Nat.leb_gt in Hab, Hba.
+apply Nat.nle_gt in Hba.
+now exfalso; apply Hba, Nat.lt_le_incl.
 Qed.
 
 Theorem Nat_ltb_antisym : antisymmetric Nat.ltb.
@@ -4090,3 +4249,29 @@ destruct fa. {
 apply sorted_cons in Hs.
 now apply IHl.
 Qed.
+
+...
+
+Compute (
+  let rel := λ a b, fst a <? fst b in
+  let la := [(1, 2); (1, 3); (1, 4)] in
+  isort rel la).
+(* not stable *)
+
+Compute (
+  let rel := λ a b, fst a <? fst b in
+  let la := [(1, 2); (1, 3); (1, 4)] in
+  bsort rel la).
+(* not stable *)
+
+Compute (
+  let rel := λ a b, fst a <? fst b in
+  let la := [(1, 2); (1, 3); (1, 4)] in
+  ssort rel la).
+(* not stable *)
+
+Compute (
+  let rel := λ a b, fst a <? fst b in
+  let la := [(1, 2); (1, 3); (1, 4)] in
+  msort rel la).
+(* not stable *)
